Prove xProps theorems for updated FFI, x \in {stack, lab, target}

compiler/backend/semantics/labSemScript.sml
@@ -371,9 +371,9 @@ val get_ret_Loc_def = Define `
 
 
 val get_carg_lab_def = Define `
-  (get_carg_lab s (C_array conf) n (SOME n') = (* with_length *)
+ (get_carg_lab s (C_array conf) n (SOME n') = (* with_length *)
     if conf.mutable then
-     (case (s.regs n,s.regs s.n') of
+     (case (s.regs n,s.regs n') of
        | (Word w, Word w') =>
         (case (read_bytearray w (w2n w') (mem_load_byte_aux s.mem s.mem_domain s.be)) of
            | SOME bytes => SOME(C_arrayv bytes)
@@ -381,32 +381,34 @@ val get_carg_lab_def = Define `
        |res => NONE)
     else NONE)
 
-/\  (get_carg_lab s (C_array conf) n NONE = (* fixed-length *)
+/\
+  (get_carg_lab s (C_array conf) n NONE = (* fixed-length *)
     if conf.mutable then
-      (case (s.regs n) of
-          | SOME (Word w) =>
-        (case (read_bytearray w 8 (*read until null terminator*) (mem_load_byte_aux s.memory s.mdomain s.be))
-               of
-                       | SOME bytes => SOME(C_arrayv bytes)
-                       | NONE => NONE)
-           | res => NONE)
+      (case s.regs n of
+        | Word w =>
+          (case (read_bytearray w 8 (*read until null terminator*) (mem_load_byte_aux s.mem s.mem_domain s.be)) of
+           | SOME bytes => SOME(C_arrayv bytes)
+           | NONE => NONE)
+        | _ => NONE)
     else NONE)
 
-/\ (get_carg_lab s  C_bool n NONE =
+/\
+  (get_carg_lab s  C_bool n NONE =
     case s.regs n of
-      | SOME (Word w) =>  if w = n2w 2 then
-      SOME(C_primv(C_boolv T))
-    else if w = n2w 18 then
-      SOME(C_primv(C_boolv F))
-    else NONE
+      | Word w =>  if w = n2w 2 then SOME(C_primv(C_boolv T))
+        else if w = n2w 18 then SOME(C_primv(C_boolv F))
+        else NONE
       | _ => NONE)
 
-/\ (get_carg_lab s C_int n NONE =
+/\
+  (get_carg_lab s C_int n NONE =
     case s.regs n of
-      | SOME (Word w) => if word_lsb w then NONE (* big num *)
-                         else SOME(C_primv(C_intv (w2i (w >>2))))
+      | Word w => if word_lsb w then NONE (* big num *)
+        else SOME(C_primv(C_intv (w2i (w >>2))))
       | _ => NONE)
-/\ (get_carg_lab _ _ _ _ = NONE)`
+
+/\
+  (get_carg_lab _ _ _ _ = NONE)`
 
 
 
@@ -417,87 +419,42 @@ val get_cargs_lab_def = Define
 /\ (get_cargs_lab _ _ _ _ = NONE)
 `
 
-
-
-val store_carg_lab_def = Define `
-  store_carg_lab w vs s = s with <| memory := write_bytearray w vs s.mem s.mem_domain s.be |>
- `
-
-val store_cargs_lab_def = Define`
-   (store_cargs_lab [] [] st = st)
-/\ (store_cargs_lab (marg::margs) (w::ws) st =
-    store_cargs_lab margs ws (store_carg_lab marg w st))
-/\ (store_cargs_lab _ _ st = st)
-`
-
-
-
-val num_word_lst_lab_def = Define `
-  (num_word_lst_lab [] s = [])
-/\
-  (num_word_lst_lab (n::ns) s = (case s.regs n of
-                                 | SOME (Word w) => SOME w :: num_word_lst_lab ns s
-                                 | NONE => NONE :: num_word_lst_stack ns s))
-`
-
-val store_cargs_nums_lab_def = Define `
-  store_cargs_nums_lab margs vs st = if (MEM NONE (num_word_lst_lab margs st)) then NONE
-                                       else SOME (store_cargs_lab (MAP THE (num_word_lst_lab margs st)) vs st)
-`
-
-val store_cargs_num'_lab_def = Define `
-  store_cargs_num'_lab margs vs n v st =
-    case (s.regs n) of
-      | SOME (Word w) => (case  mem_store w v st of
-                            | SOME st' => store_cargs_nums_lab margs vs st'
-                            | NONE => NONE)
-      | _ => NONE
+val ret_val_lab_def = Define
+`(ret_val_lab (SOME(C_boolv b)) = if b then SOME (Word (n2w 2)) else SOME (Word (n2w 18)))
+/\ (ret_val_lab (SOME(C_intv i)) = SOME (Word (Smallnum' i)))
+/\ (ret_val_lab _ = NONE)
   `
 
-
-
-
-val evaluate_ffi_def = Define `
-  evaluate_ffi s ffi_index =
-   case FIND (\x.x.mlname = ffi_index) s.ffi.signatures of
-     | SOME sign => if len_repl_ctypes sign.args <= LENGTH (s.ffi_regs) then
-       case (s.regs s.link_reg) of
-         |  Loc n1 n2 => case loc_to_pc n1 n2 s.code of
-                        | SOME new_pc =>
-          (case get_cargs_lab s sign.args (len_filter sign.args s.ffi_regs) (len_args sign.args s.ffi_regs) of
-          SOME cargs =>
-           (case call_FFI s.ffi ffi_index cargs (als_args_final_word (loc_typ_val sign.args (len_filter sign.args s.ffi_regs))) of
-            FFI_return new_ffi vs retv =>
-             if ret_ok sign.retty retv then
-                (case ret_val_word retv of
-                                | SOME v => case store_cargs_num'_lab (get_mut_args sign (len_filter sign.args s.ffi_regs)) vs s.ffi_rval v s of
-                                              | NONE => (Error,s)
-                                              | SOME s' =>  let new_io_regs = shift_seq 1 s.io_regs in
-                                                  evaluate (s' with <|
-                                                  ffi := new_ffi ;
-                                                  io_regs := new_io_regs ;
-                                                  regs := (\a. get_reg_value (s.io_regs 0 ffi_index a)
-                                                           (s.regs a) Word);
-                                                  pc := new_pc ;
-                                                  clock := s.clock - 1 |>)
-                                | NONE   => case store_cargs_num_lab (get_mut_args sign (len_filter sign.args s.ffi_regs)) vs s of
-                                              | NONE => (Error,s)
-                                              | SOME s' =>  let new_io_regs = shift_seq 1 s.io_regs in
-                                                  evaluate (s' with <|
-                                                  ffi := new_ffi ;
-                                                  io_regs := new_io_regs ;
-                                                  regs := (\a. get_reg_value (s.io_regs 0 ffi_index a)
-                                                           (s.regs a) Word);
-                                                  pc := new_pc ;
-                                                  clock := s.clock - 1 |>))
-             else (Error,s)
-        | FFI_final outcome => (Halt (FFI_outcome outcome),s))
-          | NONE => (Error,s))
-                        | _  =>  (Error,s)
-         | _ => (Error,s)
-     else (Error,s)
-     | NONE  => (Error,s)
+val get_word_margs_def = Define `
+  get_addr_margs ns s  = MAP  (\v. case v of Word w => w) (MAP (\n. s.regs n) ns)
 `
+val store_cargs_lab_def = Define
+  `(store_cargs_lab [] [] s =  s)
+/\ (store_cargs_lab (marg::margs) (w::ws) s =
+      store_cargs_lab margs ws s with <| mem := write_bytearray marg w s.mem s.mem_domain s.be |>)
+/\ (store_cargs_lab _ _ s =  s)
+  `
+
+val store_retv_cargs_lab_def = Define`
+  store_retv_cargs_lab  margs vs retv st =
+   case ret_val_lab retv of
+     | SOME v  =>  (case st.regs st.ffi_rval of
+       | Word w => if w IN st.mem_domain then
+                   SOME (store_cargs_lab margs vs (upd_mem w v st))
+                   else NONE
+       | _ => NONE)
+    | NONE => SOME (store_cargs_lab margs vs st)
+`
+
+val store_retv_cargs_lab_def = Define`
+  store_retv_cargs_lab  margs vs retv st =
+   case ret_val_lab retv of
+     | SOME v  =>  (case st.regs st.ffi_rval of
+       | Word ad => SOME (store_cargs_lab margs vs (upd_mem ad v st)) (* how to check domain etc  *)
+       | _ => NONE)
+    | NONE => SOME (store_cargs_lab margs vs st)
+`
+
 
 val evaluate_def = tDefine "evaluate" `
   evaluate (s:('a,'c,'ffi) labSem$state) =
@@ -583,35 +540,33 @@ val evaluate_def = tDefine "evaluate" `
                  | _ => (Error, s))
                  | _ => (Error, s))
         | _ => (Error, s))
-    | SOME (LabAsm (CallFFI ffi_index) _ _ _) => evaluate_ffi s ffi_index
-
-
-(*
-       (case (s.regs s.len_reg,s.regs s.ptr_reg,
-              s.regs s.len2_reg,s.regs s.ptr2_reg,s.regs s.link_reg) of
-        | (Word w, Word w2, Word w3, Word w4, Loc n1 n2) =>
-         (case (read_bytearray w2 (w2n w) (mem_load_byte_aux s.mem s.mem_domain s.be),
-                read_bytearray w4 (w2n w3) (mem_load_byte_aux s.mem s.mem_domain s.be),
-                loc_to_pc n1 n2 s.code) of
-          | (SOME bytes, SOME bytes2, SOME new_pc) =>
-             (case call_FFI s.ffi ffi_index bytes bytes2 of
-              | FFI_final outcome => (Halt (FFI_outcome outcome),s)
-              | FFI_return new_ffi new_bytes =>
-                  let new_io_regs = shift_seq 1 s.io_regs in
-                  let new_m = write_bytearray w4 new_bytes s.mem s.mem_domain s.be in
-                    evaluate (s with <|
-                                   mem := new_m ;
-                                   ffi := new_ffi ;
-                                   io_regs := new_io_regs ;
-                                   regs := (\a. get_reg_value (s.io_regs 0 ffi_index a)
-                                                  (s.regs a) Word);
-                                   pc := new_pc ;
-                                   clock := s.clock - 1 |>))
-          | _ => (Error,s))
-        | _ => (Error,s))
-
-*)
-
+    | SOME (LabAsm (CallFFI ffi_index) _ _ _) =>
+ (case FIND (\x.x.mlname = ffi_index) (debug_sig::s.ffi.signatures) of
+     | SOME sign =>
+       if len_repl_ctypes sign.args <= LENGTH (s.ffi_regs) then
+         (case (s.regs s.link_reg) of
+           | Loc n1 n2 =>
+             (case loc_to_pc n1 n2 s.code of
+               | SOME new_pc =>
+                 (case get_cargs_lab s sign.args (get_args sign.args s.ffi_regs) (get_len sign.args s.ffi_regs) of
+                   | SOME cargs => (case call_FFI s.ffi ffi_index sign cargs (als_args sign.args (get_args sign.args s.ffi_regs)) of
+                     | SOME (FFI_final outcome) => (Halt (FFI_outcome outcome),s)
+                     | SOME (FFI_return new_ffi vs retv) =>
+                       (case store_retv_cargs_lab (get_addr_margs (get_mut_args sign.args (get_args sign.args s.ffi_regs)) s) vs retv s of
+                         | NONE => (Error,s)
+                         | SOME s' => let new_io_regs  =  shift_seq 1 s.io_regs in
+                           evaluate (s' with <|
+                           ffi := new_ffi ;
+                           io_regs := new_io_regs ;
+                           regs := (\a. get_reg_value (s.io_regs 0 ffi_index a) (s.regs a) Word);
+                           pc := new_pc ;
+                           clock := s.clock - 1 |>))
+                     | NONE => (Error,s))
+                   | NONE => (Error,s))
+               | NONE  =>  (Error,s))
+           | _ => (Error,s))
+       else (Error,s)
+     | NONE => (Error,s))
     | _ => (Error,s)`
  (WF_REL_TAC `measure (\s. s.clock)`
   \\ fs [inc_pc_def] \\ rw [] \\ IMP_RES_TAC asm_fetch_IMP
